Stabilize EverCrypt.Autoconfig2

providers/evercrypt/fst/EverCrypt.AutoConfig2.fst
@@ -107,52 +107,131 @@ let recall () =
   B.recall user_wants_openssl;
   B.recall user_wants_bcrypt
 
-#set-options "--z3rlimit 500"
+inline_for_extraction noextract
+val init_aesni_flags: unit -> Stack unit
+  (requires (fun _ -> requires SC.vale))
+  (ensures (fun h0 _ h1 ->
+    B.modifies (fp_cpu_flags ()) h0 h1))
+
+let init_aesni_flags () =
+  if Vale.Wrapper.X64.Cpuid.check_aesni () <> 0UL then begin
+    B.recall cpu_has_aesni;
+    B.upd cpu_has_aesni 0ul true;
+    B.recall cpu_has_pclmulqdq;
+    B.upd cpu_has_pclmulqdq 0ul true
+  end
+
+inline_for_extraction noextract
+val init_shaext_flags: unit -> Stack unit
+  (requires (fun _ -> requires SC.vale))
+  (ensures (fun h0 _ h1 ->
+    B.modifies (fp_cpu_flags ()) h0 h1))
+
+let init_shaext_flags () =
+  if Vale.Wrapper.X64.Cpuid.check_sha () <> 0UL then begin
+    B.recall cpu_has_shaext;
+    B.upd cpu_has_shaext 0ul true
+  end
+
+inline_for_extraction noextract
+val init_avx_flags: unit -> Stack unit
+  (requires (fun _ -> requires SC.vale))
+  (ensures (fun h0 _ h1 ->
+    B.modifies (fp_cpu_flags ()) h0 h1))
+
+let init_avx_flags () =
+  if Vale.Wrapper.X64.Cpuid.check_avx () <> 0UL then begin
+    B.recall cpu_has_avx;
+    B.upd cpu_has_avx 0ul true
+  end
+
+inline_for_extraction noextract
+val init_avx2_flags: unit -> Stack unit
+  (requires (fun _ -> requires SC.vale))
+  (ensures (fun h0 _ h1 ->
+    B.modifies (fp_cpu_flags ()) h0 h1))
+
+let init_avx2_flags () =
+  if Vale.Wrapper.X64.Cpuid.check_avx2 () <> 0UL then begin
+    B.recall cpu_has_avx2;
+    B.upd cpu_has_avx2 0ul true
+  end
+
+inline_for_extraction noextract
+val init_adx_bmi2_flags: unit -> Stack unit
+  (requires (fun _ -> requires SC.vale))
+  (ensures (fun h0 _ h1 ->
+    B.modifies (fp_cpu_flags ()) h0 h1))
+
+let init_adx_bmi2_flags () =
+  if Vale.Wrapper.X64.Cpuid.check_adx_bmi2 () <> 0UL then begin
+    B.recall cpu_has_bmi2;
+    B.upd cpu_has_bmi2 0ul true;
+    B.recall cpu_has_adx;
+    B.upd cpu_has_adx 0ul true
+  end
+
+inline_for_extraction noextract
+val init_sse_flags: unit -> Stack unit
+  (requires (fun _ -> requires SC.vale))
+  (ensures (fun h0 _ h1 ->
+    B.modifies (fp_cpu_flags ()) h0 h1))
+
+let init_sse_flags () =
+  if Vale.Wrapper.X64.Cpuid.check_sse () <> 0UL then begin
+    B.recall cpu_has_sse;
+    B.upd cpu_has_sse 0ul true
+  end
+
+inline_for_extraction noextract
+val init_movbe_flags: unit -> Stack unit
+  (requires (fun _ -> requires SC.vale))
+  (ensures (fun h0 _ h1 ->
+    B.modifies (fp_cpu_flags ()) h0 h1))
+
+let init_movbe_flags () =
+  if Vale.Wrapper.X64.Cpuid.check_movbe () <> 0UL then begin
+    B.recall cpu_has_movbe;
+    B.upd cpu_has_movbe 0ul true
+  end
+
+inline_for_extraction noextract
+val init_rdrand_flags: unit -> Stack unit
+  (requires (fun _ -> requires SC.vale))
+  (ensures (fun h0 _ h1 ->
+    B.modifies (fp_cpu_flags ()) h0 h1))
+
+let init_rdrand_flags() =
+  if Vale.Wrapper.X64.Cpuid.check_rdrand () <> 0UL then begin
+    B.recall cpu_has_rdrand;
+    B.upd cpu_has_rdrand 0ul true
+  end
+
+inline_for_extraction noextract
+val init_cpu_flags: unit -> Stack unit
+  (requires (fun _ -> True))
+  (ensures (fun h0 _ h1 ->
+    B.modifies (fp_cpu_flags ()) h0 h1))
+
+let init_cpu_flags () =
+  if EverCrypt.TargetConfig.x64 then
+    if SC.vale then begin
+      init_aesni_flags ();
+      init_shaext_flags ();
+      init_adx_bmi2_flags();
+      init_avx_flags ();
+      init_avx2_flags ();
+      init_sse_flags ();
+      init_movbe_flags ();
+      init_rdrand_flags ()
+    end
+
+#set-options "--z3rlimit 50"
 let init () =
   // TODO: use an && here once macros are improved
   let h0 = ST.get () in
-  if EverCrypt.TargetConfig.x64 then
-    if SC.vale then begin
-      if Vale.Wrapper.X64.Cpuid.check_aesni () <> 0UL then begin
-        B.recall cpu_has_aesni;
-        B.upd cpu_has_aesni 0ul true;
-        B.recall cpu_has_pclmulqdq;
-        B.upd cpu_has_pclmulqdq 0ul true
-      end;
-      if Vale.Wrapper.X64.Cpuid.check_sha () <> 0UL then begin
-        B.recall cpu_has_shaext;
-        B.upd cpu_has_shaext 0ul true
-      end;
-      if Vale.Wrapper.X64.Cpuid.check_avx () <> 0UL then begin
-        B.recall cpu_has_avx;
-        B.upd cpu_has_avx 0ul true
-      end;
-      if Vale.Wrapper.X64.Cpuid.check_avx2 () <> 0UL then begin
-        B.recall cpu_has_avx2;
-        B.upd cpu_has_avx2 0ul true
-      end;
-      if Vale.Wrapper.X64.Cpuid.check_adx_bmi2 () <> 0UL then begin
-        B.recall cpu_has_bmi2;
-        B.upd cpu_has_bmi2 0ul true;
-        B.recall cpu_has_adx;
-        B.upd cpu_has_adx 0ul true
-      end;
-      if Vale.Wrapper.X64.Cpuid.check_sse () <> 0UL then begin
-        B.recall cpu_has_sse;
-        B.upd cpu_has_sse 0ul true
-      end;
-      if Vale.Wrapper.X64.Cpuid.check_movbe () <> 0UL then begin
-        B.recall cpu_has_movbe;
-        B.upd cpu_has_movbe 0ul true
-      end;
-      if Vale.Wrapper.X64.Cpuid.check_rdrand () <> 0UL then begin
-        B.recall cpu_has_rdrand;
-        B.upd cpu_has_rdrand 0ul true
-      end
-    end;
+  init_cpu_flags();
   let h1 = ST.get () in
-  assert (B.modifies (fp_cpu_flags ()) h0 h1);
-  assert (B.loc_includes (fp ()) (fp_cpu_flags()));
   assert (B.modifies (fp()) h0 h1);
   B.recall user_wants_hacl;
   B.upd user_wants_hacl 0ul SC.hacl;
